WIP

nondeterministic_dataflow/Timely_Operators.thy
@@ -7,17 +7,23 @@ begin
 
 datatype ('c, 'd) subgraph = 
   "apply": Logic "'c \<Rightarrow> (nat, nat, 'd) op"
-  | Seq "nat \<Rightarrow> 'd buf" "('c, 'd) subgraph" "('c, 'd) subgraph"
+  | Seq "nat \<Rightarrow> nat option" "nat \<Rightarrow> 'd buf" "('c, 'd) subgraph" "('c, 'd) subgraph"
 
-inductive activate where
+(* inductive activate where
   "step io (l c) (l' c') \<Longrightarrow> activate io c (Logic l) c' (Logic l')"
 | "activate (Out p x) c sg1 c' sg1' \<Longrightarrow>
    activate Tau c (Seq buf sg1 sg2) c' (Seq (BENQ p x buf) sg1' sg2)" 
+ *)
+
+fun embed_nat where
+  "embed_nat (Inl n) =  2 * n"
+| "embed_nat (Inr n) =  2 * n + 1"
 
 fun compile_subgraph where
   "compile_subgraph c (Logic l) = l c"
-| "compile_subgraph c (Seq buf sg1 sg2) = map_op projl projr (comp_op Some buf (compile_subgraph c sg1) (compile_subgraph c sg2))"
+| "compile_subgraph c (Seq wire buf sg1 sg2) = map_op embed_nat embed_nat (comp_op wire buf (compile_subgraph c sg1) (compile_subgraph c sg2))"
 
+(* 
 lemma
   "activate io c sg c' sg' \<Longrightarrow>
    step io (compile_subgraph c sg) (compile_subgraph c' sg')"
@@ -30,19 +36,61 @@ lemma
      apply simp_all
     apply (rule step_Tau_comp_op_L)
        apply simp_all
-    oops
-   
+    oops *)
 
-      find_theorems comp_op Tau Out
+inductive wactivate where
+  "step io (l c) (l' c') \<Longrightarrow> wactivate io c (Logic l) c' (Logic l')"
+| "wactivate (Out p x) c sg1 c' sg1' \<Longrightarrow>
+   wire p = Some q \<Longrightarrow>
+   wactivate Tau c sg2 c' sg2 \<Longrightarrow>
+   wactivate Tau c (Seq wire buf sg1 sg2) c' (Seq wire (BENQ q x buf) sg1' sg2)"
+ | "wactivate (Inp p x) c sg2 c' sg2' \<Longrightarrow>
+   BHD p buf = x \<Longrightarrow> buf p \<noteq> [] \<Longrightarrow>
+   p \<in> ran wire \<Longrightarrow>
+   wactivate Tau c sg1 c' sg1' \<Longrightarrow>
+   wactivate Tau c (Seq wire buf sg1 sg2) c' (Seq wire (BTL p buf) sg1' sg2')" 
+ | "wactivate (Inp p x) c sg1 c' sg1' \<Longrightarrow>
+   wactivate Tau c sg2 c' sg2' \<Longrightarrow>
+   wactivate (Inp (2 * p) x) c (Seq wire buf sg1 sg2) c' (Seq wire buf sg1' sg2')"  
+
+lemma wstep_trans_taus:
+  "wstep io op op' \<Longrightarrow> wstep Tau op' op'' \<Longrightarrow> wstep io op op''"
+  apply simp
+  apply (metis (no_types, opaque_lifting) relcomppI relcompp_assoc rtranclp_idemp rtranclp_tranclp_absorb tranclp_unfold_left wstep_def)
+  done
+
+lemma wstep_Inp_comp_op:
+  "wstep (Inp p x) op1 op1' \<Longrightarrow>
+   wstep Tau op2 op2' \<Longrightarrow>
+   wstep (Inp (2 * p) x) (map_op embed_nat embed_nat (comp_op wire buf op1 op2)) (map_op embed_nat embed_nat (comp_op wire buf op1' op2'))"
+  apply (rule wstep_map_op)
+   apply (rule wstep_trans_taus)
+    apply (rule wstep_comp_op_L_Inp)
+      apply assumption
+     apply simp_all
+  apply blast
+  done
+
+lemma
+  "wactivate io c sg c' sg' \<Longrightarrow>
+   wstep io (compile_subgraph c sg) (compile_subgraph c' sg')"
+  apply (induct io c sg c' sg'  pred: wactivate)
+  subgoal for io l c l' c'
+    apply (rule step_wstep)
+    apply simp
+    done
+  subgoal for p x c sg1 c' sg1' sg2 buf
+    apply simp
+      apply (metis (mono_tags, lifting) rtranclp_trans step_comp_op_R_Taus step_star_map_op wstep_Tau_comp_op_L wstep_steps_Tau)
+    done
+  subgoal for p x c sg2 c' sg2' buf sg1 sg1'
+    apply simp
+    apply (metis (mono_tags, lifting) rtranclp_trans step_comp_op_L_Taus step_star_map_op wstep_Tau_comp_op_R wstep_steps_Tau)
+  done
+  subgoal for p x c sg1 c' sg1' sg2 sg2' buf
+    by (simp add: wstep_Inp_comp_op)
+  done
 
 
 
-
-
-
-
-
-
-
-   
 end
